bytestring: Style fixes

theories/prelude/bytestring.v
@@ -10,14 +10,16 @@ From stdpp Require Import countable strings namespaces.
 
 (** bytes *)
 Instance byte_inhabited : Inhabited Byte.byte := populate Byte.x00.
-Instance byte_dec : EqDecision Byte.byte := Byte.byte_eq_dec.
+Instance byte_eq_dec : EqDecision Byte.byte := Byte.byte_eq_dec.
+
+#[deprecated(since="2021-09-21", note="Use [byte_eq_dec]")]
+Notation byte_dec := byte_eq_dec.
 
 Instance byte_countable : Countable Byte.byte.
 Proof.
   apply (inj_countable Byte.to_N Byte.of_N).
   abstract (by intros []).
 Defined.
-
 
 Definition byte_parse (b : Byte.byte) : Byte.byte := b.
 Definition byte_print (b : Byte.byte) : Byte.byte := b.
@@ -31,87 +33,74 @@ String Notation Byte.byte byte_parse byte_print : byte_scope.
 
 Bind Scope byte_scope with Byte.byte.
 
-Lemma byte_cmp_refl : forall a, byte_cmp a a = Eq.
+Lemma byte_cmp_refl a : byte_cmp a a = Eq.
 Proof. intros. apply N.compare_refl. Qed.
 
 Lemma byte_to_N_inj x y : Byte.to_N x = Byte.to_N y <-> x = y.
 Proof.
-  split.
-  2: destruct 1; reflexivity.
-  intros.
-  assert (Some x = Some y).
-  { do 2 rewrite <- Byte.of_to_N.
-    destruct H. reflexivity. }
-  injection H0. auto.
+  split. 2: now intros ->.
+  intros Heq.
+  enough (Some x = Some y) as [= ->] by easy.
+  do 2 rewrite <- Byte.of_to_N.
+  now rewrite Heq.
 Qed.
 
 Module OT_byte <: OrderedType.OrderedType with Definition t := Byte.byte.
   Definition t := Byte.byte.
   Definition eq := fun l r => byte_cmp l r = Eq.
   Definition lt := fun l r => byte_cmp l r = Lt.
-  Theorem eq_refl : ∀ x : t, eq x x.
+  Theorem eq_refl (x : t) : eq x x.
   Proof.
     intros; apply N.compare_refl.
   Qed.
-  Theorem eq_sym : ∀ x y : t, eq x y → eq y x.
+  Theorem eq_sym (x y : t) : eq x y -> eq y x.
   Proof.
-    intros. eapply N.compare_eq in H. red. unfold byte_cmp.
-    destruct H. apply eq_refl.
+    intros Hxy. eapply N.compare_eq in Hxy. unfold eq, byte_cmp.
+    rewrite Hxy. apply eq_refl.
   Qed.
-  Theorem eq_trans : ∀ x y z : t, eq x y → eq y z → eq x z.
+  Theorem eq_trans (x y z : t) : eq x y -> eq y z -> eq x z.
   Proof.
-    intros. eapply N.compare_eq in H. eapply N.compare_eq in H0.
-    red. unfold byte_cmp.
-    destruct H. destruct H0. apply eq_refl.
+    intros Hxy Hyz. eapply N.compare_eq in Hxy. eapply N.compare_eq in Hyz.
+    unfold eq, byte_cmp. rewrite -> Hxy, Hyz.
+    apply eq_refl.
   Qed.
-  Theorem lt_trans : ∀ x y z : t, lt x y → lt y z → lt x z.
+  Theorem lt_trans (x y z : t) : lt x y -> lt y z -> lt x z.
   Proof.
-    unfold lt, byte_cmp.
-    intros.
-    rewrite ->N.compare_lt_iff in H.
-    rewrite ->N.compare_lt_iff in H0.
-    rewrite N.compare_lt_iff.
+    unfold lt, byte_cmp. rewrite ->!N.compare_lt_iff.
     lia.
   Qed.
-  Theorem lt_not_eq : ∀ x y : t, lt x y → ¬ eq x y.
+  Theorem lt_not_eq (x y : t) : lt x y -> ~ eq x y.
   Proof.
-    unfold lt, eq, byte_cmp; intros.
-    rewrite ->N.compare_lt_iff in H.
-    rewrite N.compare_eq_iff.
+    unfold lt, eq, byte_cmp. rewrite ->N.compare_lt_iff, N.compare_eq_iff.
     lia.
   Qed.
   Definition compare (x y : t) : OrderedType.Compare lt eq x y.
-    refine  (
-    match byte_cmp x y as X return byte_cmp x y = X -> OrderedType.Compare lt eq x y  with
-    | Eq => fun pf => OrderedType.EQ pf
-    | Lt => fun pf => OrderedType.LT pf
-    | Gt => fun pf => OrderedType.GT _
-    end (Logic.eq_refl)).
+  Proof.
+    refine (match byte_cmp x y as X return byte_cmp x y = X -> OrderedType.Compare lt eq x y with
+      | Eq => fun pf => OrderedType.EQ pf
+      | Lt => fun pf => OrderedType.LT pf
+      | Gt => fun pf => OrderedType.GT _
+      end Logic.eq_refl).
     unfold lt, byte_cmp.
     abstract (rewrite N.compare_antisym; apply CompOpp_iff, pf).
   Defined.
 
-  Definition eq_dec : ∀ x y : t, {eq x y} + {¬ eq x y}.
+  Definition eq_dec (x y : t) : {eq x y} + {~ eq x y}.
   Proof.
-  unfold eq.
-  refine (fun x y =>
-      match byte_cmp x y as Z return byte_cmp x y = Z -> _ with
-      | Eq => fun pf => left pf
-      | _ => fun _ => right _
-      end Logic.eq_refl);
-  abstract congruence.
+    refine (match byte_cmp x y as Z return byte_cmp x y = Z -> _ with
+        | Eq => fun pf => left pf
+        | _ => fun _ => right _
+        end Logic.eq_refl);
+    abstract congruence.
   Defined.
-
 End OT_byte.
 
-Theorem byte_cmp_spec : forall x y, CompareSpec (x = y) (OT_byte.lt x y) (OT_byte.lt y x) (byte_cmp x y).
+Theorem byte_cmp_spec x y : CompareSpec (x = y) (OT_byte.lt x y) (OT_byte.lt y x) (byte_cmp x y).
 Proof.
-  intros. unfold byte_cmp.
-  unfold OT_byte.lt, byte_cmp.
+  unfold byte_cmp, OT_byte.lt, byte_cmp.
   destruct (N.compare_spec (Byte.to_N x) (Byte.to_N y)); constructor; auto.
   apply byte_to_N_inj. assumption.
 Qed.
-
 
 (** bytestrings *)
 (** Many functions on byte strings are meant to be always used
@@ -120,10 +109,12 @@ qualified, as they conflict with similar functions from [List] or [String].
 All such functions are collected in a module [BS], which is not meant
 to be imported, as it defines names like [t].
 *)
+
 Module Import BS.
   Inductive t : Set :=
   | EmptyString
   | String (_ : Byte.byte) (_ : t).
+
   Definition eq_dec (x y : t) : {x = y} + {x <> y}.
   Proof. decide equality. apply Byte.byte_eq_dec. Defined.
 
@@ -139,15 +130,15 @@ Module Import BS.
     | b :: bs => String b (parse bs)
     end.
 
-  Lemma print_parse_inv:
-    ∀ x : BS.t, BS.parse (BS.print x) = x.
+  Lemma print_parse_inv (x : BS.t) :
+    BS.parse (BS.print x) = x.
   Proof.
     induction x; simpl; intros; auto.
     f_equal; auto.
   Qed.
 
-  Lemma parse_print_inv:
-    ∀ x : list Byte.byte, BS.print (BS.parse x) = x.
+  Lemma parse_print_inv (x : list Byte.byte) :
+    BS.print (BS.parse x) = x.
   Proof.
     induction x; simpl; intros; auto.
     f_equal; auto.
@@ -276,16 +267,15 @@ Module Import BS.
     | String _ l => S (length l)
     end.
 
-  Lemma print_length :
-    forall (s : bs),
-      List.length (BS.print s) = BS.length s.
+  Lemma print_length (s : bs) :
+    List.length (BS.print s) = BS.length s.
   Proof.
-    intros s; induction s; intros *; simpl.
+    induction s; simpl.
     - done.
     - by rewrite IHs.
   Qed.
 
-  Fixpoint contains (start: nat) (keys: list bs) (fullname: bs) :bool :=
+  Fixpoint contains (start : nat) (keys : list bs) (fullname : bs) :bool :=
     match keys with
     | kh::ktl =>
       match index start kh fullname with
@@ -320,9 +310,9 @@ Module OT_bs <: OrderedType.OrderedType with Definition t := bs.
   Definition eq := @eq bs.
   Definition lt := fun l r => bs_cmp l r = Lt.
 
-  Theorem lm : forall x y, CompareSpec (x = y) (lt x y) (lt y x) (bs_cmp x y).
+  Theorem lm x y : CompareSpec (x = y) (lt x y) (lt y x) (bs_cmp x y).
   Proof.
-    induction x; destruct y; simpl.
+    revert y; induction x; destruct y; simpl.
     - constructor; reflexivity.
     - constructor. reflexivity.
     - constructor. reflexivity.
@@ -338,30 +328,25 @@ Module OT_bs <: OrderedType.OrderedType with Definition t := bs.
 
   Definition compare (x y : t) : OrderedType.Compare lt eq x y.
   Proof.
-    refine  (
-    match bs_cmp x y as X return bs_cmp x y = X -> OrderedType.Compare lt eq x y  with
-    | Eq => fun pf => OrderedType.EQ _
-    | Lt => fun pf => OrderedType.LT pf
-    | Gt => fun pf => OrderedType.GT _
-    end (Logic.eq_refl));
+    refine (
+      match bs_cmp x y as X return bs_cmp x y = X -> OrderedType.Compare lt eq x y  with
+      | Eq => fun pf => OrderedType.EQ _
+      | Lt => fun pf => OrderedType.LT pf
+      | Gt => fun pf => OrderedType.GT _
+      end (Logic.eq_refl));
     abstract (generalize (lm x y); rewrite pf; inversion 1; auto).
   Defined.
 
-  Theorem eq_refl : ∀ x : t, eq x x.
-  Proof.
-    reflexivity.
-  Qed.
-  Theorem eq_sym : ∀ x y : t, eq x y → eq y x.
-  Proof.
-    eapply eq_sym.
-  Qed.
-  Theorem eq_trans : ∀ x y z : t, eq x y → eq y z → eq x z.
-  Proof.
-    eapply eq_trans.
-  Qed.
-  Theorem lt_trans : ∀ x y z : t, lt x y → lt y z → lt x z.
+  Theorem eq_refl (x : t) : eq x x.
+  Proof. reflexivity. Qed.
+  Theorem eq_sym (x y : t) : eq x y -> eq y x.
+  Proof. eapply eq_sym. Qed.
+  Theorem eq_trans (x y z : t) : eq x y -> eq y z -> eq x z.
+  Proof. eapply eq_trans. Qed.
+  Theorem lt_trans (x y z : t) : lt x y -> lt y z -> lt x z.
   Proof.
     unfold lt.
+    revert y z.
     induction x; destruct y; simpl; try congruence.
     - destruct z; congruence.
     - destruct (byte_cmp_spec b b0); subst.
@@ -379,12 +364,12 @@ Module OT_bs <: OrderedType.OrderedType with Definition t := bs.
         * congruence.
       + congruence.
   Qed.
-  Theorem lt_not_eq : ∀ x y : t, lt x y → ¬ eq x y.
+  Theorem lt_not_eq (x y : t) : lt x y -> ~ eq x y.
   Proof.
     unfold lt, eq.
-    intros. intro. subst.
+    intros Heq ->.
     induction y; simpl in *; try congruence.
-    rewrite ->byte_cmp_refl in *. auto.
+    rewrite ->byte_cmp_refl in Heq. auto.
   Qed.
 
   Definition eq_dec := BS.eq_dec.
